
% -------------------------------------------------------------------------

\documentclass{article}
\usepackage{float}
\usepackage[margin=1.5in]{geometry} % Please keep the margins at 1.5 so that there is space for grader comments.
\usepackage{amsmath,amsthm,amssymb,hyperref}
\usepackage{algorithmic}
%\usepackage[options ]{algorithm2e}
\usepackage{algorithm2e}
\usepackage{dsfont}
\newcommand{\R}{\mathbf{R}}  
\newcommand{\Z}{\mathbf{Z}}
\newcommand{\N}{\mathbf{N}}
\newcommand{\Q}{\mathbf{Q}}
\DeclareMathOperator{\qp}{q_\pi} % indicates the the q vlaue function following policy pi
\DeclareMathOperator{\vp}{v_\pi} % value funciton following policy pi
\DeclareMathOperator{\rhp}{\rho_{\pi}} % the probability fgunciton for following policy pi
\DeclareMathOperator{\state}{\mathcal{S}}
\DeclareMathOperator{\action}{\mathcal{A}}
\DeclareMathOperator{\reward}{\mathcal{R}}
\DeclareMathOperator{\E}{\mathds{E}}
\DeclareMathOperator{\Ep}{\E_\pi}
\DeclareMathOperator{\vpd}{v_{\pi'}}
\DeclareMathOperator{\qpd}{q_{\pi'}}
\DeclareMathOperator{\maxa}{\underset{a}{\text{max }}}
\DeclareMathOperator{\dynamics}{\sum_{s',r} p(s',r|s,a)}
\DeclareMathOperator{\argmaxa}{\underset{a}{\text{argmax }}}
\newenvironment{theorem}[2][Theorem]{\begin{trivlist}
\item[\hskip \labelsep {\bfseries #1}\hskip \labelsep {\bfseries #2.}]}{\end{trivlist}}
\newenvironment{lemma}[2][Lemma]{\begin{trivlist}
\item[\hskip \labelsep {\bfseries #1}\hskip \labelsep {\bfseries #2.}]}{\end{trivlist}}
\newenvironment{claim}[2][Claim]{\begin{trivlist}
\item[\hskip \labelsep {\bfseries #1}\hskip \labelsep {\bfseries #2.}]}{\end{trivlist}}
\newenvironment{problem}[2][Problem]{\begin{trivlist}
\item[\hskip \labelsep {\bfseries #1}\hskip \labelsep {\bfseries #2.}]}{\end{trivlist}}
\newenvironment{proposition}[2][Proposition]{\begin{trivlist}
\item[\hskip \labelsep {\bfseries #1}\hskip \labelsep {\bfseries #2.}]}{\end{trivlist}}
\newenvironment{corollary}[2][Corollary]{\begin{trivlist}
\item[\hskip \labelsep {\bfseries #1}\hskip \labelsep {\bfseries #2.}]}{\end{trivlist}}

\newenvironment{solution}{\begin{proof}[Solution]}{\end{proof}}

\begin{document}

\large % please keep the text at this size for ease of reading.


{  % Replace with appropriate page number 
\hfill Dhawal Gupta}

\begin{center}
Extra Parts\end{center}
\vspace{0.05in}

% -----------------------------------------------------
% The "enumerate" environment allows for automatic problem numbering.
% To make the number for the next problem, type " \item ". 
% To make sub-problems such as (a), (b), etc., use an "enumerate" within an "enumerate."
% -----------------------------------------------------
\section{Proofs}
\subsection{Proof of $\vp(s)$}
\begin{align*}
	\vp(s) &= \Ep[G_t | S_t = s] \\
	&= \Ep [R_{t+1} + \gamma G_{t+1} | S_t = s]\\
	&= \Ep[R_{t+1}  | S_t= s] + \gamma \Ep[G_{t+1} | S_t= s]\\
	&= \sum_{r,  a} r \times \pi(a|s) \times p(r|s,a) + \gamma  \Ep[G_{t+1} | S_t= s]\\
	&= \sum_{r,  a} r \pi(a|s)  p(r|s,a) +\\
	& \gamma  ( \sum_{s'}( \sum_a \pi(a|s)p(s'|s,a)  \Ep[G_{t+1} | S_{t+1} = s']))\\
	&= \sum_a \pi(a|s) [  \sum_r r p(r|s,a) + \\
	&\gamma \sum_{s'}p(s'|s,a) \Ep[G_{t+1} | S_{t+1} = s']  ]\\
	&= \sum_a \pi(a|s) [  \sum_{r,s'} r p(s',r|s,a) +\\
	& \gamma \sum_{s',r}p(s',r|s,a) \Ep[G_{t+1} | S_{t+1} = s']  ]\\
	&= \sum_a \pi(a|s) \sum_{r,s'} p(s',r|s,a)[ r + \gamma \Ep[G_{t+1} | S_{t+1} = s']  ]\\
	&= \sum_a \pi(a|s) \sum_{s',r} p(s',r|s,a) [r + \gamma \vp(s')] \forall s \in \state
\end{align*}
\subsection{Proof of Policy Improvement}
\begin{align*}
	\vp(s) & \leq \qp(s,\pi'(s))\\
	&= \E_{R_{t+1},S_{t+1} \sim p(s',r|s,a) }[ R_{t+1}+ \gamma \vp(S_{t+1}) | S_t = s, A_t = \pi'(s)]\\
	&= \E_{R_{t+1},S_{t+1} \sim p(s',r|s,a) ,a \sim \pi'}[ R_{t+1}+ \gamma \vp(S_{t+1}) | S_t = s]\\
	& \text{ Shortening the notation}\\
	&= \E_{\pi'}[ R_{t+1}+ \gamma \vp(S_{t+1}) | S_t = s]\\
	& \text{Applying $\pi'$ on another step we get}\\
	& \leq  \E_{\pi'}[ R_{t+1} + \gamma \qp(S_{t+1}, \pi'(S_{t+1}) | S_t = s]\\
	& = \E_{\pi'}[ R_{t+1} + \gamma  \E_{\pi'}[R_{t+2} + \gamma \vp(S_{t+2}) | S_{t+1}]    | S_t = s]\\
	& = \E_{\pi'} [ R_{t+1} | S_t = s]+ \gamma   \E_{\pi'} [ \E_{\pi'}[R_{t+2} + \gamma \vp(S_{t+2}) | S_{t+1}]    | S_t = s]\\
	& =  \sum_a \pi'(a|s) \sum_{r} p(r|s,a) r + \gamma   \sum_a \pi'(a|s) \sum_{s'} p(s'|s,a)\E_{\pi'}[R_{t+2} + \gamma \vp(S_{t+2}) | S_{t+1} = s']    \\
	& =  \sum_a \pi'(a|s) \sum_{s',r} p(s',r|s,a) r + \gamma   \sum_a \pi'(a|s) \sum_{s',r} p(s',r|s,a)\E_{\pi'}[R_{t+2} + \gamma \vp(S_{t+2}) | S_{t+1} = s']    \\
	& =  \sum_a \pi'(a|s) \sum_{s',r} p(s',r|s,a)  ( r + \gamma \E_{\pi'}[R_{t+2} + \gamma \vp(S_{t+2}) | S_{t+1} = s']   )\\
	& \text{expanding the inside expectation just like the outside}\\
	& =  \sum_a \pi'(a|s) \sum_{s',r} p(s',r|s,a)  ( r + \gamma\sum_a \pi'(a'|s') \sum_{s'',r'} p(s'',r'|s',a')  ( r' + \gamma \vp(s'') )   )\\
	& \text{ as we know $\sum_{a'} \pi'(a'|s') \sum_{s'',r'} p(s'',r'|s',a') = \sum_{a',s'',r'} p_{\pi'}(a',r',s'' | s') = 1$}\\
	&\text{ and not dependent on $r$}\\
	& =  \sum_a \pi'(a|s) \sum_{s',r} p(s',r|s,a)  ( \sum_{a'} \pi'(a'|s')  \sum_{s'',r'} p(s'',r'|s',a') r + \\
	& \qquad \gamma\sum_{a'} \pi'(a'|s') \sum_{s'',r'} p(s'',r'|s',a')  ( r' + \gamma \vp(s'') )   )\\
	& =  \sum_a \pi'(a|s) \sum_{s',r} p(s',r|s,a)  \sum_{a'} \pi'(a'|s')  \sum_{s'',r'} p(s'',r'|s',a') (r +  \gamma  ( r' + \gamma \vp(s'') )   )\\
	& =  \sum_a \pi'(a|s) \sum_{s',r} p(s',r|s,a)  \sum_{a'} \pi'(a'|s')  \sum_{s'',r'} p(s'',r'|s',a') (r +  \gamma  r' + \gamma^2 \vp(s'') )   )\\
	& = \sum_{a,s',r} p_{\pi'}(s',r,a|s ) \sum_{a',s'',r'} p_{\pi'}(s'',r',a'|s' )(r +  \gamma  r' + \gamma^2 \vp(s'') )   )\\
	&  \text{ as internal expression is not dependent on $a$ and $a'$ we can sum on them}\\
	\end{align*}
\begin{align*}
	& = \sum_{s',r} p_{\pi'}(s',r|s ) \sum_{s'',r'} p_{\pi'}(s'',r'|s' ) (r +  \gamma  r' + \gamma^2 \vp(s'') ) )\\
	& = \sum_{r, s',r', s''} p_{\pi'}(s',r|s ) p_{\pi'}(s'',r'|s' ) (r +  \gamma  r' + \gamma^2 \vp(s'') ) )\\
	& \text{ we can write this in terms of $a,b,c,d,e$ for ease of readbaility}\\
	& = p(a,b | c) p(d, e | a)= p(a|b, c) p(b|c) p(d, e|a) \\
	& = \sum_{r, s',r', s''} p_{\pi'}(s'|r,s ) p_{\pi'}(r|s) p_{\pi'}(s'',r'|s' ) (r +  \gamma  r' + \gamma^2 \vp(s'') ) )\\
	& \text{ we can write $p_{\pi'}(s'',r'|s' ) = p_{\pi'}(s'',r'|s' , s, r)$ }\\& \quad \text{as its markov they are equal as they are not dependent on $s$ and $r$ and only on $s'$}\\
	& = \sum_{r, s',r', s''} p_{\pi'}(s'|r,s ) p_{\pi'}(r|s) p_{\pi'}(s'',r'|s' , s, r) (r +  \gamma  r' + \gamma^2 \vp(s'') ) )\\
	& = \sum_{r, s',r', s''}  p_{\pi'}(r|s) p_{\pi'}(s'',r',s'|  s, r) (r +  \gamma  r' + \gamma^2 \vp(s'') ) )\\
	& = \sum_{r, s',r', s''}   p_{\pi'}(s'',r',s', r|  s) (r +  \gamma  r' + \gamma^2 \vp(s'') ) )\\
	& \text{ we can sum on $s'$ as the independent expression doesnt containt hat term}\\
	& = \sum_{r,r', s''}   p_{\pi'}(s'',r', r|  s) (r +  \gamma  r' + \gamma^2 \vp(s'') ) )\\
	& = \E_{\pi'} [R_{t+1} + \gamma R_{t+2} + \gamma^2 \vp(S_{t+2}) | S_t = s]
\end{align*}



% ---------------------------------------------------
% Anything after the \end{document} will be ignored by the typesetting.
% ----------------------------------------------------

\end{document}

